Integrate new canon with slprops. Correctness to prove

pulse/examples/steel/NewCanon.fst
@@ -2,6 +2,12 @@ module NewCanon
 
 open FStar.Tactics
 
+open Steel.Memory
+
+let is_uvar (t:term) : Tac bool = match t with
+  | Tv_Uvar _ _ -> true
+  | _ -> false
+
 (* For a given term t, collect all terms in the list l with the same head symbol *)
 let rec get_candidates (t:term) (l:list term) : Tac (list term) =
   let name, _ = collect_app t in
@@ -32,15 +38,10 @@ let rec trivial_cancels (l1 l2:list term)
   match l1 with
   | [] -> [], l2, [], []
   | hd::tl ->
-      let b, l2'   = trivial_cancel  hd l2 in
+      let b, l2'   = trivial_cancel hd l2 in
       let l1', l2', l1_del, l2_del = trivial_cancels tl l2' in
       (if b then l1' else hd::l1'), l2',
       (if b then hd::l1_del else l1_del), (if b then hd::l2_del else l2_del)
-
-let rec dump_terms (l:list term) : Tac unit =
-  match l with
-  | [] -> dump "end"; ()
-  | hd::tl -> dump (term_to_string hd); dump_terms tl
 
 exception Failed
 exception Success
@@ -50,7 +51,6 @@ let rec try_candidates (t:term) (l:list term) : Tac (term * int) =
   match l with
   | [] -> t, 0
   | hd::tl ->
-      dump (term_to_string hd);
       // Encapsulate unify in a try/with to ensure unification is not actually performed
       let res = try if unify t hd then raise Success else raise Failed
                 with | Success -> true | _ -> false in
@@ -100,10 +100,12 @@ let rec equivalent_lists' (n:nat) (l1 l2 l1_del l2_del:list term)
   match l1 with
   | [] -> begin match l2 with
     | [] -> dump "equiv"; (l1_del, l2_del)
-    | _ ->
-      // TODO: This should succeed if l2 only contains uvars or emp,
-      //as it can be unified with emp
-      dump "not equiv"; (l1_del, l2_del)
+    | [hd] ->
+      // Succeed if there is only one uvar left in l2, which can be therefore
+      // be unified with emp
+      if is_uvar hd then (dump "equiv with remaining emp uvar"; ((`emp)::l1_del, hd::l2_del))
+      else (dump "not equiv"; (l1_del, l2_del))
+    | _ -> dump "not equiv"; (l1_del, l2_del)
     end
   | _ ->
     let rem1, rem2, l1_del', l2_del' = equivalent_lists_once l1 l2 l1_del l2_del in
@@ -121,31 +123,333 @@ let equivalent_lists (l1 l2:list term) : Tac (list term * list term) =
   let l1_del, l2_del = equivalent_lists' n l1 l2 l1_del l2_del in
   l1_del, l2_del
 
+open FStar.Reflection.Derived.Lemmas
+
+let rec list_to_string (l:list term) : Tac string =
+  match l with
+  | [] -> "end"
+  | hd::tl -> term_to_string hd ^ " " ^ list_to_string tl
+
+
+noeq
+type exp : Type =
+  | Unit : exp
+  | Mult : exp -> exp -> exp
+  | Atom : term -> exp
+
+let rec reification_aux (mult unit t:term) : Tac (exp * list term) =
+  let hd, tl = collect_app_ref t in
+  match inspect hd, List.Tot.Base.list_unref tl with
+  | Tv_FVar fv, [(t1, Q_Explicit) ; (t2, Q_Explicit)] ->
+    if term_eq (pack (Tv_FVar fv)) mult
+    then (let (e1, ts1) = reification_aux mult unit t1 in
+          let (e2, ts2) = reification_aux mult unit t2 in
+          (Mult e1 e2, ts1 `List.Tot.append` ts2))
+    else Atom t, [t]
+  | _, _ ->
+    if term_eq t unit
+    // Do not add emps to the list of slprops
+    then (Unit, [])
+    else Atom t, [t]
+
+
+let reification (eq: term) (m: term) (t:term) :
+    Tac (exp * list term) =
+  let open FStar.Algebra.CommMonoid.Equiv in
+  let mult = norm_term [iota; zeta; delta] (`CM?.mult (`#m)) in
+  let unit = norm_term [iota; zeta; delta] (`CM?.unit (`#m)) in
+  let t    = norm_term [iota; zeta] t in
+  reification_aux mult unit t
+
+
+let canon_l_r (eq: term) (m: term) (lhs rhs:term) : Tac unit =
+  let open FStar.Algebra.CommMonoid.Equiv in
+  let m_unit = norm_term [iota; zeta; delta](`CM?.unit (`#m)) in
+  let (r1, ts1) = reification eq m lhs in
+  let (r2, ts2) = reification eq m rhs in
+  dump (list_to_string ts1);
+  dump (list_to_string ts2);
+  dump "ending";
+  let l1, l2 = equivalent_lists ts1 ts2 in
+  ()
+
+
+let canon_monoid (eq:term) (m:term) : Tac unit =
+  norm [iota; zeta];
+  let t = cur_goal () in
+  // removing top-level squash application
+  let sq, rel_xy = collect_app_ref t in
+  // unpacking the application of the equivalence relation (lhs `EQ?.eq eq` rhs)
+  (match rel_xy with
+   | [(rel_xy,_)] -> (
+       let open FStar.List.Tot.Base in
+       let rel, xy = collect_app_ref rel_xy in
+       if (length xy >= 2)
+       then (
+         match index xy (length xy - 2) , index xy (length xy - 1) with
+         | (lhs, Q_Explicit) , (rhs, Q_Explicit) ->
+           canon_l_r eq m lhs rhs
+         | _ -> fail "Goal should have been an application of a binary relation to 2 explicit arguments"
+       )
+       else (
+         fail "Goal should have been an application of a binary relation to n implicit and 2 explicit arguments"
+       )
+     )
+   | _ -> fail "Goal should be squash applied to a binary relation")
+
 #set-options "--print_implicits"
 
-assume val p (#n:int) (n2:int) : Type
-assume val q (#n:int) (#n':int) (n2:int) : Type
+
+(* Try to integrate it into larger tactic *)
+
+open Steel.FramingEffect
+
+let canon' () : Tac unit =
+  canon_monoid (`Steel.Memory.Tactics.req) (`Steel.Memory.Tactics.rm)
+
+let solve_can_be_split (args:list argv) : Tac bool =
+  match args with
+  | [(t1, _); (t2, _)] ->
+      let lnbr = slterm_nbr_uvars t1 in
+      let rnbr = slterm_nbr_uvars t2 in
+      if lnbr + rnbr <= 1 then (
+        let open FStar.Algebra.CommMonoid.Equiv in
+        focus (fun _ -> norm [delta_only [`%can_be_split]];
+                     // If we have exactly the same term on both side,
+                     // equiv_sl_implies would solve the goal immediately
+                     or_else (fun _ -> apply_lemma (`lemma_sl_implies_refl))
+                      (fun _ -> apply_lemma (`equiv_sl_implies);
+                       norm [delta_only [
+                              `%__proj__CM__item__unit;
+                              `%__proj__CM__item__mult;
+                              `%Steel.Memory.Tactics.rm;
+                              `%__proj__Mktuple2__item___1; `%__proj__Mktuple2__item___2;
+                              `%fst; `%snd];
+                            primops; iota; zeta];
+                       dump "can_be_split";
+                       canon'()));
+        true
+      ) else false
+
+  | _ -> false // Ill-formed can_be_split, should not happen
+
+let solve_can_be_split_forall (args:list argv) : Tac bool =
+  match args with
+  | [_; (t1, _); (t2, _)] ->
+      let lnbr = slterm_nbr_uvars t1 in
+      let rnbr = slterm_nbr_uvars t2 in
+      if lnbr + rnbr <= 1 then (
+        let open FStar.Algebra.CommMonoid.Equiv in
+        focus (fun _ -> ignore (forall_intro());
+                     norm [delta_only [`%can_be_split_forall]];
+                     or_else (fun _ -> apply_lemma (`lemma_sl_implies_refl))
+                       (fun _ ->
+                       apply_lemma (`equiv_sl_implies);
+                       or_else (fun _ ->  flip()) (fun _ -> ());
+                       norm [delta_only [
+                              `%__proj__CM__item__unit;
+                              `%__proj__CM__item__mult;
+                              `%Steel.Memory.Tactics.rm;
+                              `%__proj__Mktuple2__item___1; `%__proj__Mktuple2__item___2;
+                              `%fst; `%snd];
+                            primops; iota; zeta];
+                       dump "can_be_split_forall";
+                       canon'()));
+        true
+      ) else false
+
+  | _ -> false // Ill-formed can_be_split, should not happen
+
+let rec solve_subcomp_post (l:list goal) : Tac unit =
+  match l with
+  | [] -> ()
+  | hd::tl ->
+    let f = term_as_formula' (goal_type hd) in
+    match f with
+    | App _ t ->
+        let hd, args = collect_app t in
+        if term_eq hd (quote annot_sub_post) then (focus (fun _ ->
+          norm [delta_only [`%annot_sub_post]];
+          // Assuming for now that the body will always be Steel
+          // instead of SteelF, as we'll lift pure to Steel by
+          // a polymonadic bind with Steel alloc/read/...
+          // That means the postcondition of return will be ?u_ret * ?u_emp
+          or_else (fun _ -> apply_lemma (`emp_unit_variant))
+                  (fun _ ->
+                     norm [delta_only [`%can_be_split_forall]];
+                     ignore (forall_intro());
+                     or_else
+                       (fun _ -> apply_lemma (`lemma_sl_implies_refl))
+                       (fun _ ->
+                       let open FStar.Algebra.CommMonoid.Equiv in
+                       apply_lemma (`equiv_sl_implies);
+                       or_else (fun _ ->  flip()) (fun _ -> ());
+                       norm [delta_only [
+                              `%__proj__CM__item__unit;
+                              `%__proj__CM__item__mult;
+                              `%Steel.Memory.Tactics.rm;
+                              `%__proj__Mktuple2__item___1; `%__proj__Mktuple2__item___2;
+                              `%fst; `%snd];
+                            primops; iota; zeta];
+                       dump "subcomp";
+                       canon'()))
+          ))
+        else (later());
+        solve_subcomp_post tl
+    | _ -> later(); solve_subcomp_post tl
+
+let is_return_eq (l r:term) : Tac bool =
+  let nl, al = collect_app l in
+  let nr, ar = collect_app r in
+  match al, ar with
+  | [(t1, _)], [(t2, _)] ->
+    let b1 = is_uvar nl in
+    let b2 = is_uvar nr in
+    let b3 = not (is_uvar t1) in
+    let b4 = not (is_uvar t2) in
+    b1 && b2 && b3 && b4
+  | _ -> false
+
+let rec solve_indirection_eqs (l:list goal) : Tac unit =
+  match l with
+  | [] -> ()
+  | hd::tl ->
+    let f = term_as_formula' (goal_type hd) in
+    match f with
+    | Comp (Eq _) l r ->
+        if is_return_eq l r then later() else trefl();
+        solve_indirection_eqs tl
+    | _ -> later(); solve_indirection_eqs tl
+
+let rec solve_triv_eqs (l:list goal) : Tac unit =
+  match l with
+  | [] -> ()
+  | hd::tl ->
+    let f = term_as_formula' (goal_type hd) in
+    match f with
+    | Comp (Eq _) l r ->
+      let lnbr = slterm_nbr_uvars l in
+      let rnbr = slterm_nbr_uvars r in
+      // Only solve equality if there is only one uvar
+      // trefl();
+     if lnbr = 0 || rnbr = 0 then trefl () else later();
+      solve_triv_eqs tl
+    | _ -> later(); solve_triv_eqs tl
+
+// Returns true if the goal has been solved, false if it should be delayed
+let solve_or_delay (g:goal) : Tac bool =
+  let f = term_as_formula' (goal_type g) in
+  match f with
+  | App _ t ->
+      let hd, args = collect_app t in
+      if term_eq hd (quote delay) then false
+      else if term_eq hd (quote can_be_split) then solve_can_be_split args
+      else if term_eq hd (quote can_be_split_forall) then solve_can_be_split_forall args
+      else false
+  | Comp (Eq _) l r ->
+    let lnbr = slterm_nbr_uvars l in
+    let rnbr = slterm_nbr_uvars r in
+    // Only solve equality if one of the terms is completely determined
+    if lnbr = 0 || rnbr = 0 then (trefl (); true) else false
+  | _ -> false
+
+
+// Returns true if it successfully solved a goal
+// If it returns false, it means it didn't find any solvable goal,
+// which should mean only delayed goals are left
+let rec pick_next (l:list goal) : Tac bool =
+  match l with
+  | [] -> false
+  | a::q -> if solve_or_delay a then true else (later (); pick_next q)
+
+let rec resolve_tac () : Tac unit =
+  match goals () with
+  | [] -> ()
+  | g ->
+    if pick_next g then resolve_tac ()
+    else
+      (norm [delta_only [`%delay]];
+      resolve_tac ())
+
+let typ_contains_req_ens (t:term) : Tac bool =
+  let name, _ = collect_app t in
+  if term_eq name (`req_t) || term_eq name (`ens_t) then true
+  else false
+
+let rec filter_goals (l:list goal) : Tac (list goal * list goal) =
+  match l with
+  | [] -> [], []
+  | hd::tl ->
+      let slgoals, loggoals = filter_goals tl in
+      match term_as_formula' (goal_type hd) with
+      | Comp (Eq t) _ _ ->
+        if Some? t then
+          let b = typ_contains_req_ens (Some?.v t) in
+          if b then slgoals, hd::loggoals
+          else hd::slgoals, loggoals
+        else hd::slgoals, loggoals
+      | App t _ -> if term_eq t (`squash) then hd::slgoals, loggoals else slgoals, loggoals
+      | _ -> slgoals, loggoals
+
+[@@ resolve_implicits; framing_implicit]
+let init_resolve_tac () : Tac unit =
+  let slgs, loggs = filter_goals (goals()) in
+  set_goals slgs;
+  // We first need to solve the trivial equalities to ensure we're not restricting
+  // scopes for annotated slprops
+  solve_triv_eqs (goals ());
+  solve_indirection_eqs (goals());
+  solve_subcomp_post (goals ());
+  resolve_tac ();
+  set_goals loggs;
+  resolve_tac ()
+
+assume val p (#n:int) (n2:int) : slprop
+assume val q (#n:int) (#n':int) (n2:int) : slprop
+
+assume val palloc (#n:int) (n2:int) : SteelT unit emp (fun _ -> p #n n2)
 
 let l:list int = [0; 1; 2]
 
-let rec string_of_list (l:list term) = match l with
+let rec string_of_list (l:list slprop) = match l with
   | [] -> ""
-  | a::q -> term_to_string a ^ " " ^ string_of_list q
+  | a::q -> term_to_string (`a) ^ " " ^ string_of_list q
 
-let _ =
-  let terms:list term =
-//    [(`p #0 1); (`p #2 1); (`p #1 0); (`q #1 #2 1); (`q #_ #3 1)] in
-    [(`p #0 1); (`p #2 1); (`p #1 0); (`q #_ #3 1); (`q #1 #2 1); (`p #2 2)] in
-  let p_terms:list term =
-    // A uvar is also added at the head in the assert .. by
-    [(`p #2 1); (`p #_ 0); (`p #_ 1); (`q #_ #3 1); (`q #_ #_ 1)] in
-  // The assertion fails because implicits are not unified in this case,
-  // but the important part is the result of equivalent_lists, given as
-  // a dump in the tactic.
-  assert (True) by (
-    let u = fresh_uvar None in
-    let l1_del, l2_del = equivalent_lists terms (u::p_terms) in
-    dump (string_of_list l1_del);
-    dump (string_of_list l2_del)
-    );
-  ()
+
+assume val ref : Type0
+assume val ptr (_:ref) : slprop u#1
+
+assume val alloc (x:int)  : SteelT ref emp (fun y -> ptr y)
+assume val free (r:ref) : SteelT unit (ptr r) (fun _ -> emp)
+assume val read (r:ref) : SteelT int (ptr r) (fun _ -> ptr r)
+
+
+
+let test1 (x:int) : SteelT unit emp (fun _ -> p #1 1)  =
+  let _ = palloc #_ 1 in ()
+
+
+// let f (#r:slprop) =
+//   let terms:slprop =
+//     (p #0 1) `star` (p #2 1) in
+// //    [(`p #0 1); (`p #2 1); (`p #1 0); (`q #1 #2 1); (`q #_ #3 1)] in
+// //    [(p #0 1); (p #2 1); (p #1 0); (q #i1 #3 1); (q #1 #2 1); (p #2 2)] in
+//   let p_terms:slprop =
+//     (p #0 1) `star` (p #i1 1) in
+//     // A uvar is also added at the head in the assert .. by
+// //    [(`p #2 1); (`p #_ 0); (`p #_ 1); (`q #_ #3 1); (`q #_ #_ 1)] in
+//   // The assertion fails because implicits are not unified in this case,
+//   // but the important part is the result of equivalent_lists, given as
+//   // a dump in the tactic.
+//   assert (terms `equiv` p_terms) by (
+// //    let u = fresh_uvar (Some (`slprop)) in
+//     // dump (string_of_list [r]);
+//     // dump (string_of_list terms);
+//     dump "test";
+//     apply_lemma (`equiv_symmetric);
+//     dump "here"
+//     // let l1_del, l2_del = equivalent_lists terms (r::p_terms) in
+//     // dump (string_of_list l1_del);
+//     // dump (string_of_list l2_del)
+//     );
+//   ()
